ocaml/fstar-lib/generated/FStar_Parser_Const.ml
@@ -105,6 +105,10 @@ let (list_append_lid : FStar_Ident.lident) = p2l ["FStar"; "List"; "append"]
 let (list_tot_append_lid : FStar_Ident.lident) =
   p2l ["FStar"; "List"; "Tot"; "Base"; "append"]
 let (id_lid : FStar_Ident.lident) = psconst "id"
+let (seq_cons_lid : FStar_Ident.lident) =
+  p2l ["FStar"; "Seq"; "Base"; "cons"]
+let (seq_empty_lid : FStar_Ident.lident) =
+  p2l ["FStar"; "Seq"; "Base"; "empty"]
 let (c2l : Prims.string -> FStar_Ident.lident) =
   fun s -> p2l ["FStar"; "Char"; s]
 let (char_u32_of_char : FStar_Ident.lident) = c2l "u32_of_char"
